nlist_assoc_sorted

src/lowparse/LowParse.SteelST.Assoc.fst
@@ -690,4 +690,244 @@ let nlist_assoc_default_eq_keys
 
 (* If we know that the list of keys is sorted with a transitive order, then we can interrupt the search as soon as the key in the map is (strictly) greater than the key we are looking for. *)
 
+module I16 = FStar.Int16
 
+inline_for_extraction
+let nlist_assoc_compare_keys
+  (#kkey: Ghost.erased parser_kind)
+  (#tkey: Type)
+  (pkey: parser kkey tkey)
+  (key_order: Ghost.erased (tkey -> tkey -> bool))
+  (key: Ghost.erased tkey)
+  (rkey: vprop)
+: Tot Type
+= (#va: v kkey tkey) ->
+  (a: byte_array) ->
+  (sz: SZ.t) ->
+  ST I16.t
+    (rkey `star` aparse pkey a va)
+    (fun _ -> rkey `star` aparse pkey a va)
+    (SZ.v sz == AP.length (array_of va))
+    (fun res -> 
+      (res = 0s <==> Ghost.reveal key == va.contents) /\
+      (res `I16.lt` 0s <==> Ghost.reveal key_order key va.contents)
+    )
+
+#push-options "--z3rlimit 32 --split_queries always"
+
+#restart-solver
+inline_for_extraction
+let nlist_assoc_sorted_step
+  (#kkey: Ghost.erased parser_kind)
+  (#tkey: Type)
+  (#pkey: parser kkey tkey)
+  (jump_key: jumper pkey)
+  (#kvalue: Ghost.erased parser_kind)
+  (#tvalue: Type)
+  (#pvalue: parser kvalue tvalue)
+  (jump_value: jumper pvalue)
+  (#key: Ghost.erased tkey)
+  (#rkey: vprop)
+  (#key_order: Ghost.erased (tkey -> tkey -> bool))
+  (compare_keys: nlist_assoc_compare_keys pkey key_order key rkey)
+  (key_order_irrefl: (
+    (k1: tkey) ->
+    (k2: tkey) ->
+    Lemma
+    (requires (Ghost.reveal key_order k1 k2))
+    (ensures (~ (k1 == k2)))
+  ))
+  (key_order_trans: (
+    (k1: tkey) ->
+    (k2: tkey) ->
+    (k3: tkey) ->
+    Lemma
+    (requires (Ghost.reveal key_order k1 k2 /\ Ghost.reveal key_order k2 k3))
+    (ensures (Ghost.reveal key_order k1 k3))
+  ))
+  (n0: Ghost.erased nat)
+  (va0: v (parse_nlist_kind n0 (and_then_kind kkey kvalue)) (nlist n0 (tkey & tvalue)))
+  (a0: byte_array)
+  (pa: R.ref byte_array)
+  (pn: R.ref SZ.t)
+  (pres: R.ref byte)
+  (_: unit)
+: STT unit
+    (nlist_assoc_invariant pkey pvalue key rkey (Some (Ghost.reveal key_order)) n0 va0 a0 pa pn pres true)
+    (fun _ -> exists_ (nlist_assoc_invariant pkey pvalue key rkey (Some (Ghost.reveal key_order)) n0 va0 a0 pa pn pres))
+= rewrite
+    (nlist_assoc_invariant pkey pvalue key rkey (Some (Ghost.reveal key_order)) n0 va0 a0 pa pn pres true)
+    (nlist_assoc_invariant0 pkey pvalue key rkey (Some (Ghost.reveal key_order)) n0 va0 a0 pa pn pres true);
+  let _ = gen_elim () in
+  let n = read_replace pn in
+  let n_pred = n `SZ.sub` 1sz in
+  rewrite
+    (nlist_assoc_invariant_aux pkey pvalue key rkey (Some (Ghost.reveal key_order)) n0 va0 a0 pa _ _)
+    (nlist_assoc_invariant_aux_continue pkey pvalue key rkey (Some (Ghost.reveal key_order)) n0 va0 a0 pa (SZ.v n));
+  let _ = gen_elim () in
+  let a = read_replace pa in
+  vpattern_rewrite (fun a -> aparse _ a _) a;
+  let va = vpattern_replace (fun va -> aparse _ a va `star` nlist_iterator (pkey `nondep_then` pvalue) (n0) va0 a0 (SZ.v n) va) in
+  nlist_iterator_parser_kind _ _ _ _ _ _;
+  let ga' = elim_nlist_cons _ (SZ.v n) (SZ.v n_pred) a in
+  let _ = gen_elim () in
+  let gav = g_split_pair pkey pvalue a in
+  let _ = gen_elim () in
+  let key_size = get_parsed_size jump_key a in
+  let av = hop_aparse_aparse_with_size pkey pvalue a key_size gav in
+  let res = compare_keys a key_size in
+  if res = 0s
+  then begin
+    R.write pa av;
+    R.write pres nlist_assoc_success;
+    let vav = vpattern_replace (aparse pvalue av) in
+    intro_implies
+      (aparse pvalue av vav)
+      (aparse (parse_nlist (n0) (pkey `nondep_then` pvalue)) a0 va0)
+      (aparse pkey a _ `star` aparse _ ga' _ `star` nlist_iterator (pkey `nondep_then` pvalue) (n0) va0 a0 (SZ.v n) va)
+      (fun _ ->
+        let _ = merge_pair pkey pvalue a av in
+        let _ = intro_nlist_cons (SZ.v n) (pkey `nondep_then` pvalue) (SZ.v n_pred) a ga' in
+        vpattern_rewrite (aparse _ a) va;
+        nlist_iterator_end _ _ _
+      );
+    rewrite
+      (nlist_assoc_post_success pkey pvalue key rkey (n0) va0 a0 pa)
+      (nlist_assoc_invariant_aux pkey pvalue key rkey (Some (Ghost.reveal key_order)) n0 va0 a0 pa (SZ.v n) nlist_assoc_success);
+    rewrite
+      (nlist_assoc_invariant0 pkey pvalue key rkey (Some (Ghost.reveal key_order)) n0 va0 a0 pa pn pres false)
+      (nlist_assoc_invariant pkey pvalue key rkey (Some (Ghost.reveal key_order)) n0 va0 a0 pa pn pres false);
+    return ()
+  end else if res `I16.lt` 0s
+  then begin
+    let vak = vpattern (aparse pkey a) in
+    let vav = vpattern (aparse pvalue av) in
+    let va' : v _ (nlist (SZ.v n_pred) _) = vpattern_replace (aparse (parse_nlist (SZ.v n_pred) (pkey `nondep_then` pvalue)) ga') in
+    map_entry_order_assoc_order_none key_order key_order_irrefl key_order_trans vak.contents vav.contents va'.contents (Ghost.reveal key);
+    R.write pres nlist_assoc_failure;
+    let _ = merge_pair pkey pvalue a av in
+    let _ = intro_nlist_cons (SZ.v n) (pkey `nondep_then` pvalue) (SZ.v n_pred) a ga' in
+    vpattern_rewrite (aparse _ a) va;
+    nlist_iterator_end _ _ _;
+    rewrite
+      (nlist_assoc_post_failure pkey pvalue key rkey (n0) va0 a0 pa)
+      (nlist_assoc_invariant_aux pkey pvalue key rkey (Some (Ghost.reveal key_order)) n0 va0 a0 pa (SZ.v n) nlist_assoc_failure);
+    rewrite
+      (nlist_assoc_invariant0 pkey pvalue key rkey (Some (Ghost.reveal key_order)) n0 va0 a0 pa pn pres false)
+      (nlist_assoc_invariant pkey pvalue key rkey (Some (Ghost.reveal key_order)) n0 va0 a0 pa pn pres false);
+    return ()
+  end else begin
+    let a' = hop_aparse_aparse jump_value (parse_nlist (SZ.v n_pred) (pkey `nondep_then` pvalue)) av ga' in
+    R.write pa a';
+    R.write pn n_pred;
+    let va' = vpattern_replace (aparse _ a') in
+    let _ = merge_pair pkey pvalue a av in
+    nlist_iterator_next (pkey `nondep_then` pvalue) #n0 #va0 a0 a #(SZ.v n_pred) va';
+    noop ();
+    rewrite
+      (nlist_assoc_invariant_aux_continue pkey pvalue key rkey (Some (Ghost.reveal key_order)) n0 va0 a0 pa (SZ.v n_pred))
+      (nlist_assoc_invariant_aux pkey pvalue key rkey (Some (Ghost.reveal key_order)) n0 va0 a0 pa (SZ.v n_pred) nlist_assoc_in_progress);
+    intro_nlist_assoc_invariant pkey pvalue key rkey (Some (Ghost.reveal key_order)) n0 va0 a0 pa pn pres (n_pred <> 0sz) _ _;
+    return ()
+  end
+
+#pop-options
+
+inline_for_extraction
+let nlist_assoc_sorted
+  (#kkey: Ghost.erased parser_kind)
+  (#tkey: Type)
+  (#pkey: parser kkey tkey)
+  (jump_key: jumper pkey)
+  (#kvalue: Ghost.erased parser_kind)
+  (#tvalue: Type)
+  (#pvalue: parser kvalue tvalue)
+  (jump_value: jumper pvalue)
+  (#key: Ghost.erased tkey)
+  (#rkey: vprop)
+  (#key_order: Ghost.erased (tkey -> tkey -> bool))
+  (compare_keys: nlist_assoc_compare_keys pkey key_order key rkey)
+  (key_order_irrefl: (
+    (k1: tkey) ->
+    (k2: tkey) ->
+    Lemma
+    (requires (Ghost.reveal key_order k1 k2))
+    (ensures (~ (k1 == k2)))
+  ))
+  (key_order_trans: (
+    (k1: tkey) ->
+    (k2: tkey) ->
+    (k3: tkey) ->
+    Lemma
+    (requires (Ghost.reveal key_order k1 k2 /\ Ghost.reveal key_order k2 k3))
+    (ensures (Ghost.reveal key_order k1 k3))
+  ))
+  (n0: SZ.t)
+  (#va0: v (parse_nlist_kind (SZ.v n0) (and_then_kind kkey kvalue)) (nlist (SZ.v n0) (tkey & tvalue)))
+  (a0: byte_array)
+  (pa: R.ref byte_array)
+: ST bool
+    (rkey `star`
+      aparse (parse_nlist (SZ.v n0) (pkey `nondep_then` pvalue)) a0 va0 `star`
+      (exists_ (R.pts_to pa full_perm))
+    )
+    (fun res ->
+      nlist_assoc_post pkey pvalue key rkey (SZ.v n0) va0 a0 pa res
+    )
+    (kkey.parser_kind_subkind == Some ParserStrong /\
+      kvalue.parser_kind_subkind == Some ParserStrong /\
+      List.Tot.sorted (map_entry_order key_order tvalue) va0.contents
+    )
+    (fun _ -> True)
+= let _ = gen_elim () in
+  R.write pa a0;
+  let _ = nlist_iterator_begin (pkey `nondep_then` pvalue) #(SZ.v n0) a0 in
+  with_local n0 (fun pn ->
+    with_local nlist_assoc_in_progress (fun pres ->
+      noop ();
+      rewrite
+        (nlist_assoc_invariant_aux_continue pkey pvalue key rkey (Some (Ghost.reveal key_order)) (SZ.v n0) va0 a0 pa (SZ.v n0))
+        (nlist_assoc_invariant_aux pkey pvalue key rkey (Some (Ghost.reveal key_order)) (SZ.v n0) va0 a0 pa (SZ.v n0) nlist_assoc_in_progress);
+      rewrite
+        (nlist_assoc_invariant0 pkey pvalue key rkey (Some (Ghost.reveal key_order)) (SZ.v n0) va0 a0 pa pn pres (n0 <> 0sz))
+        (nlist_assoc_invariant pkey pvalue key rkey (Some (Ghost.reveal key_order)) (SZ.v n0) va0 a0 pa pn pres (n0 <> 0sz));
+      Steel.ST.Loops.while_loop
+        (nlist_assoc_invariant pkey pvalue key rkey (Some (Ghost.reveal key_order)) (SZ.v n0) va0 a0 pa pn pres)
+        (nlist_assoc_invariant_test pkey pvalue key rkey (Some (Ghost.reveal key_order)) (SZ.v n0) va0 a0 pa pn pres)
+        (nlist_assoc_sorted_step jump_key jump_value compare_keys key_order_irrefl key_order_trans (SZ.v n0) va0 a0 pa pn pres);
+      let _ = nlist_assoc_invariant_end pkey pvalue key rkey (Some (Ghost.reveal key_order)) (SZ.v n0) va0 a0 pa pn pres in
+      let _ = gen_elim () in
+      let res = R.read pres in
+      vpattern_rewrite (nlist_assoc_post pkey pvalue key rkey (SZ.v n0) va0 a0 pa) (res = nlist_assoc_success);
+      noop ();
+      return (res = nlist_assoc_success)
+  ))
+
+(* This type is useful only to determine whether a map is sorted along
+   its key. It is useless in the context of querying for a map entry
+ *)
+
+inline_for_extraction
+let map_entry_order_impl
+  (#kkey: Ghost.erased parser_kind)
+  (#key: Type0)
+  (pkey: parser kkey key)
+  (#key_order: Ghost.erased (key -> key -> bool))
+  (key_order_impl: order_impl pkey key_order)
+  (#kvalue: Ghost.erased parser_kind)
+  (#value: Type0)
+  (pvalue: parser kvalue value)
+: Pure (order_impl (pkey `nondep_then` pvalue) (map_entry_order key_order value))
+    (requires (kkey.parser_kind_subkind == Some ParserStrong))
+    (ensures (fun _ -> True))
+= fun #va1 #va2 a1 a2 ->
+    let av1 = g_split_pair pkey pvalue a1 in
+    let _ = gen_elim () in
+    let av2 = g_split_pair pkey pvalue a2 in
+    let _ = gen_elim () in
+    let res = key_order_impl a1 a2 in
+    let _ = merge_pair pkey pvalue a1 av1 in
+    vpattern_rewrite (aparse _ a1) va1;
+    let _ = merge_pair pkey pvalue a2 av2 in
+    vpattern_rewrite (aparse _ a2) va2;
+    return res
